code/theories/ReductionConfluence.v
@@ -1,0 +1,174 @@
+From Interpolation Require Import Utils Syntax Notations Elim Reduction.
+
+(** ** Confluence of commuting conversion *)
+
+Section CommutConfluence.
+  Context `{l : Lang}.
+
+  Close Scope typing_scope.
+
+  (** *** Commuting conversion *)
+  Inductive commut : relation term :=
+
+    | C_Comm_Abort e t :
+      zip e (tAbort t) ⤳ tAbort t
+
+    | C_Comm_If e s bl br :
+      zip e (tIf s bl br) ⤳ tIf s (zip e⟨↑⟩ bl) (zip e⟨↑⟩ br)
+
+    (** congruences *)
+    | C_Lam t t' :
+      t ⤳ t' ->
+      tLam t ⤳ tLam t'
+    | C_App_l t1 t1' t2 :
+          t1 ⤳ t1' ->
+          tApp t1 t2 ⤳ tApp t1' t2
+    | C_App_r t1 t2 t2' :
+          t2 ⤳ t2' ->
+          tApp t1 t2 ⤳ tApp t1 t2'
+    | C_Proj b t t' :
+          t ⤳ t' ->
+          tProj b t ⤳ tProj b t'
+    | C_Pair_l t1 t1' t2 :
+          t1 ⤳ t1' ->
+          tPair t1 t2 ⤳ tPair t1' t2
+    | C_Pair_r t1 t2 t2' :
+          t2 ⤳ t2' ->
+          tPair t1 t2 ⤳ tPair t1 t2'
+    | C_Abort t t' :
+        t ⤳ t' ->
+        tAbort t ⤳ tAbort t'
+    | C_In b t t' :
+      t ⤳ t' ->
+      tIn b t ⤳ tIn b t'
+    | C_If_s s s' bl br :
+      s ⤳ s' ->
+      tIf s bl br ⤳ tIf s' bl br
+    | C_If_l s bl bl' br :
+      bl ⤳ bl' ->
+      tIf s bl br ⤳ tIf s bl' br
+    | C_If_r s bl br br' :
+      br ⤳ br' ->
+      tIf s bl br ⤳ tIf s bl br'
+
+  (** In this section we use the reduction symbol for this reduction *)
+  where "t '⤳' t'" := (commut t t').
+
+  Notation "t '⤳*' t'" := (clos_refl_trans term commut t t').
+
+  (** *** Size *)
+
+  Fixpoint size (t : term) : nat :=
+    match t with
+    | tVar _ | tStar | tConst _ => 1
+    | tPair p q => 1 + size p + size q
+    | tProj _ p => 1 + 3*(size p)
+    | tLam t => 1 + size t
+    | tApp f u => 1 + (size f)*(3 + size u)
+    | tAbort t => 1 + 3*(size t)
+    | tIn _ t => 1 + (size t)
+    | tIf s bl br => 1 + (size s)*(3 + size bl + size br)
+    end.
+
+  Lemma size_ren (t : term) (ρ : ren) : size (t⟨ρ⟩) = size t.
+  Proof.
+    induction t in ρ |- * ; cbn.
+    all: repeat (match goal with | IH : forall ρ, size _ = size _ |- _ => rewrite IH end).
+    all: lia.
+  Qed.
+
+  Lemma size_ren_subst (t : term) (ρ : ren) : size (t[ρ >> tVar]) = size t.
+  Proof.
+    renamify ; refold.
+    apply size_ren.
+  Qed.
+
+  Lemma size_pos (t : term) : 0 < size t.
+  Proof.
+    destruct t ; cbn ; lia.
+  Qed.
+
+  Lemma up_ren_subst (ρ : nat -> nat) : ⇑ (ρ >> tVar) =1 (⇑ ρ) >> tVar.
+  Proof.
+    asimpl ; unfold up_term_ren ; now asimpl.
+  Qed.
+
+  (** Size decreases along reductions *)
+  Lemma commut_lt (t t' : term) : t ⤳ t' -> size t' < size t.
+  Proof.
+    induction 1.
+    all: (try match goal with | e : elim |- _ => destruct e end) ;
+      cbn -[Nat.add Nat.mul] ; refold.
+    all: rewrite ?up_ren_subst, ?size_ren_subst.
+    all: try solve [nia].
+    - pose proof (size_pos t1).
+      nia.
+    - pose proof (size_pos s).
+      nia.
+    - pose proof (size_pos s).
+      nia.
+  Qed.
+
+  (** Thus the reduction is strongly normalising *)
+
+  Corollary strong_nor : well_founded (flip commut).
+  Proof.
+    eapply well_founded_lt_compat.
+    unfold flip.
+    intros *.
+    apply commut_lt.
+  Qed.
+
+  (** Local confluence is admitted *)
+  Lemma loc_confluent (t u u' : term) : t ⤳ u -> t ⤳ u' -> exists v, u ⤳* v /\ u' ⤳* v.
+  Proof.
+    (** This is proven by CSIho *)
+  Admitted.
+
+  Definition nf t := ~ (exists t', t ⤳ t').
+
+  Lemma rt_inv_l {A} {R : relation A} a a' :
+    clos_refl_trans _ R a a' ->
+    a = a' \/ exists a'', R a a'' /\ clos_refl_trans _ R a'' a'.
+  Proof.
+    intros H.
+    induction H.
+    - right.
+      now eexists.
+    - now left.
+    - destruct IHclos_refl_trans1 as [->|(?&?&?)].
+      1: easy.
+      
+      right ; eexists.
+      split ; [easy|].
+      now etransitivity.
+  Qed.
+     
+  (** We derive confluence *)
+  Lemma confluent (t u u' : term) : t ⤳* u -> t ⤳* u' -> exists v, u ⤳* v /\ u' ⤳* v.
+  Proof.
+    revert u u'.
+    pattern t.
+    revert t.
+    unshelve eapply well_founded_ind.
+    2: apply strong_nor.
+    intros t IH u u' Hred Hred'.
+    unfold flip in IH.
+    apply rt_inv_l in Hred as [<- | (t'&Hredt1&Hredt')].
+    1: now exists u'.
+    apply rt_inv_l in Hred' as [<- | (t''&Hredt2&Hredt'')].
+    1: exists u ; split ; [easy|] ; etransitivity ; tea ; now econstructor.
+    edestruct (loc_confluent t t' t'') as (v&Hredv1&Hredv2); tea.
+    unshelve epose proof (IH t' _ u v _ _) as (v'&Hredu&Hredv); tea.
+    unshelve epose proof (IH t'' _ u' v' _ _) as (v''&Hredu'&Hredv'); tea.
+    1: now etransitivity.
+    exists v'' ; split ; eauto.
+    now etransitivity.
+  Qed.
+  
+End CommutConfluence.
+
+(** We do not prove confluence of β or commutation, so we admit confluence
+  of the full reduction relation (ie containing β and commuting conversions) *)
+Axiom confluence : forall `{Lang} (t u u' : term),
+  (t ⤳* u) -> (t ⤳* u') -> exists v, (u ⤳* v) /\ (u' ⤳* v).
