README.md
@@ -1,17 +1,53 @@
 # Interpolation-STLC
 
+This is the formalisation accompanying the paper _Bidirectional Interpolation for the Lambda-Calculus_.
+
+## Installation
+
+The project builds with Rocq version `9.0`, and depends on the [`smpl`](https://github.com/uds-psl/smpl/), [Equations](https://github.com/mattam82/Coq-Equations/) and [`stdpp`](https://gitlab.mpi-sws.org/iris/stdpp/) libraries.
+If you already have an opam set-up, dependencies can be installed by simply using `opam install ./code/ --deps-only`.
+
+Once the dependencies have been installed, you can issue `make` in the `code` folder to
+build the whole development.
+
+The project uses the [AutoSubst](https://github.com/uds-psl/autosubst-ocaml) tool to generate syntax-related boilerplate, although it is not necessary to install it to build the project, as we directly include the generated files (slightly modified, see the paper for explanation).
+
+## Overview
+
+The definition of typing is in [Typing](./code/theories/Typing.v), that of reduction is in [Reduction](./code/theories/Reduction.v), and that of conversion is in [Equations](./code/theories/Equations.v). Definitions related to atoms and constants are in [Languages](./code/theories/Languages.v). The confluence axiom is in [ReductionConfluence](./code/theories/ReductionConfluence.v).
+
+The main theorems are in [Theorems](./code/theories/Theorems.v). To avoid having to compare terms in languages with different sets of constants, which would be painful (and require its own notion of substitution, etc), we instead phrase them with respect to a unique global language containing all necessary constants, and show the terms only use the appropriate constants.
+
+## Confluence
+
+We include in the `confluence` subfolder the [CSIho](http://cl-informatik.uibk.ac.at/software/csi/ho/) tool and [file](./confluence/comm_cuts.trs) we used to check confluence. The command to invoke is in the [Makefile](./confluence/Makefile), and in the output the relevant line is 
+the one saying
+```
+  critical peaks: 12, all joinable
+```
+The tool does not conclude about confluence per-se because it is unable to prove termination, which we have proven separately, in [ReductionConfluence](./code/theories/ReductionConfluence.v).
+
+## File structure
+
+All names refer to files in the `code` folder. A [dependency graph](./code/docs/dependency_graph.png) is provided in the `code/docs` subfolder.
 
 File | Content
 -----|--------
 Utils | Generic utilities
-BasicAst | Definitions on which that of syntax depends: base types, etc.
-Notations | Reserves most notations used in the project, can be used as index!
-Ast.sig | Signature of the AST of simply-typed lambda-calculus
 core, unscoped | Autosubst utilities
-Ast.v | Auto-generated from the above by Autosubst
+BasicAst | Definitions on which that of syntax depends: base types, constants, etc.
+Notations | Reserves most notations used in the project, can be used as index of notations!
 Context | Definition of context and context access
+Ast.sig | Signature of the AST of simply-typed lambda-calculus
+Ast.v | Syntax and substitution, auto-generated from the above by Autosubst
 Syntax | Notations and helpers to deal with the generated syntax
+Elim | Operations on eliminators
 Reduction | Definition and properties of reduction
+ReductionConfluence | A partial proof of confluence of commuting conversion, and the confluence axiom
 Typing | Definition and properties of (undirected) typing
 Bidir | Definition of bidirectional typing (characterising normal forms)
-Interpolation | The main theorem
+Equations | Definition and properties of conversion
+Languages | Definition and properties of the atoms/constants of a type, context, term
+MetaTheory | Meta-theoretic properties of typing, including normalisation
+Interpolation | The main inductive proof
+Theorems | “Top-level” theorems, putting together normalisation, interpolation, and properties of conversion
